notes/CodegenReasoning.md
@@ -1,0 +1,49 @@
+# Reasoning in the codegen monad
+
+Our compiler is a monadic computation. This makes it easier to reason
+about compositionally, since it's implemented using the monad's
+operations and generic combinators like ret, bind, and mapM.
+
+Here are a few rules to follow when writing lemmas about computations
+in the codegen monad so that we prove things at the right level of
+generality.
+
+## Rule 1: assume a successful run_codegen.
+The codegen monad supports exceptions. Our FTLR assumes the compiler
+succeeds and the compiler never catches its own errors, so you should never
+need to reason about the exception case. Every lemma about a
+computation `c` should take the form
+
+```
+forall wl v wl' es, 
+  run_codegen c wl = inr (v, wl', es) ->
+  ...
+```
+
+## Rule 2: constrain the return value.
+A successful computation `c : codegen A` produces a triple `(a, wl,
+es)` where `a: A`. In the conclusion of your lemma, constrain the
+value of `a`. If `A` happens to be `unit`, include `a = ()` in your
+postcondition. Generally try to give the most general specification
+for `a` you can.
+
+## Rule 3: constrain the output context.
+Likewise, for the output state/context, try to give a general spec. This will usually look like 
+```
+wl' = wl ++ new_stuff,
+```
+where `wl` was the original context.
+
+## Rule 4: constrain the Wasm code
+For the expressions `es` written by the computation, you can either
+give a syntactic postcondition or a semantic one. A syntactic
+postcondition looks like the `es = es1 ++ es2` in the conclusion of
+`run_codegen_bind_dist`. A semantic postcondition leaves the exact
+shape of `es` unconstrained and instead gives an Iris weakest
+precondition involving `es`, like the conclusion of `wp_if_c`:
+```
+WP to_e_list (BI_const (VAL_int32 i) :: es) @ s; E {{ v, Φ v }}.
+```
+Notice that this adds an argument stack to the left of `es` and (if
+you look at the full lemma) also expects some weakest preconditions
+for the true and false branches of the code as assumptions.
